1. $y_{1}=g_{1}\left(x_{1}, x_{2}\right)$ and $y_{2}=g_{2}\left(x_{1}, x_{2}\right)$ can be uniquely solved for $x_{1}$ and $x_{2}$ to get, say, $x_{1}=h_{1}\left(y_{1}, y_{2}\right), x_{2}=h_{2}\left(y_{1}, y_{2}\right)$
2. The functions $g_{1}$ and $g_{2}$ have continuous partial derivatives and the determinant of the following determinant
$$
J\left(x_{1}, x_{2}\right)=\left|\begin{array}{ll}
\frac{\partial g_{1}}{\partial x_{1}} & \frac{\partial g_{1}}{\partial x_{2}} \\
\frac{\partial g_{2}}{\partial x_{1}} & \frac{\partial g_{2}}{\partial x_{2}}
\end{array}\right| \neq 0
$$
Then $f_{Y_{1}, Y_{2}}\left(y_{1}, y_{2}\right)=f_{X_{1}, X_{2}}\left(x_{1}, x_{2}\right)\left|J\left(x_{1}, x_{2}\right)\right|^{-1}$ where
$$
x_{1}=h_{1}\left(y_{1}, y_{2}\right), x_{2}=h_{2}\left(y_{1}, y_{2}\right)
$$
Theorem Let $X$ be a continuous random variable with density function $f_{X}$. Suppose that $g(x)$ is a strictly monotone (increasing or decreasing), differentiable (and thus c

ontinuous) function of $x$. Then the random variable $Y$ defined by $Y=g(X)$ has a density function given by
要记住的是，pdf是从cdf定义出来的，所以说记得要还原成cdf
$$
f_{Y}(y)= \begin{cases}f_{X}\left[g^{-1}(y)\right]\left|\frac{d}{d y} g^{-1}(y)\right| & \text { if } y=g(x) \text { for some } x \\ 0 & \text { if } y \neq g(x) \text { for all } x\end{cases}
$$
证明 事实上, 当 $g$ 严格上升时, 有
$$
\begin{aligned}
F_{Y}(x) &=\mathbf{P}(Y \leqslant x)=\mathbf{P}(g(X) \leqslant x)=\mathbf{P}\left(X \leqslant g^{-1}(x)\right) \\
&=\mathbf{P}(X \leqslant h(x))=F_{X}(h(x)),
\end{aligned}
$$
当 $g$ 严格下降时, 有
$$
\begin{aligned}
F_{Y}(x) &=\mathbf{P}(Y \leqslant x)=\mathbf{P}(g(X) \leqslant x)=\mathbf{P}\left(X \geqslant g^{-1}(x)\right) \\
&=\mathbf{P}(X \geqslant h(x))=1-F_{X}(h(x)) .
\end{aligned}
$$
再利用关系式 $p_{Y}(x)=\frac{\mathrm{d}}{\mathrm{d} x} F_{Y}(x)$, 即可在上述两种情况下分别求得
$$
p_{Y}(x)=\frac{\mathrm{d}}{\mathrm{d} x} F_{X}(h(x))=p_{X}(h(x)) h^{\prime}(x)=p_{X}(h(x))\left|h^{\prime}(x)\right|, \quad x \in(\alpha, \beta)
$$
和
$$
p_{Y}(x)=\frac{\mathrm{d}}{\mathrm{d} x}\left\{-F_{X}(h(x))\right\}=-p_{X}(h(x)) h^{\prime}(x)=p_{X}(h(x))\left|h^{\prime}(x)\right|, \quad x \in(\alpha, \beta)
$$